generic/Zeta.HashFunction.fsti
@@ -4,4 +4,4 @@ open Zeta.Hash
 open Zeta.App
 open Zeta.Record
 
-val hashfn (#aprm: app_params) (v: value aprm): Tot hash_value
+val hashfn (#aprm: app_params) (v: value aprm): GTot hash_value
